Extraction: simplify types
Get rid of mllib, since all these lists are singletons in all we do and
we carry list of mllibs anyway. Also make the printers work on single
module at a time.

src/ml/FStarC_Extraction_ML_PrintML.ml
@@ -508,7 +508,7 @@ let build_module1 path (m1: mlmodule1): structure_item option =
       Some (Str.value Nonrecursive [binding])
   | MLM_Loc (p, f) -> None
 
-let build_m path (md: (mlsig * mlmodule) option) : structure =
+let build_m path (md: (mlsig * mlmodulebody) option) : structure =
   match md with
   | Some(s, m) ->
     let open_plugin_lib =
@@ -527,17 +527,15 @@ let build_m path (md: (mlsig * mlmodule) option) : structure =
     open_plugin_lib @ open_guts @ open_prims @ (map (build_module1 path) m |> flatmap opt_to_list)
   | None -> []
 
-let build_ast (out_dir: string option) (ext: string) (ml: mllib) =
-  match ml with
-  | MLLib l ->
-     map (fun (p, md, _) ->
-         let m = path_to_string p in
-         current_module := m;
-         let name = BatString.concat "" [m; ext] in
-         let path = (match out_dir with
-           | Some out -> BatString.concat "/" [out; name]
-           | None -> name) in
-         (path, build_m path md)) l
+let build_ast (out_dir: string option) (ext: string) (modul: mlmodule) =
+  let p, md = modul in
+  let m = path_to_string p in
+  current_module := m;
+  let name = BatString.concat "" [m; ext] in
+  let path = (match out_dir with
+    | Some out -> BatString.concat "/" [out; name]
+    | None -> name) in
+  (path, build_m path md)
 
 
 (* printing the AST to the correct path *)
@@ -547,18 +545,18 @@ let print_module ((path, m): string * structure) =
   structure Format.std_formatter m;
   Format.pp_print_flush Format.std_formatter ()
 
-let print (out_dir: string option) (ext: string) (ml: mllib) =
+let print (out_dir: string option) (ext: string) (modul: mlmodule) =
   match ext with
   | ".ml" ->
      (* Use this printer for OCaml extraction *)
-     let ast = build_ast out_dir ext ml in
-     iter print_module ast
+     let ast = build_ast out_dir ext modul in
+     print_module ast
   | ".fs" ->
      (* Use the old printer for F# extraction *)
-     let new_doc = FStarC_Extraction_ML_Code.doc_of_mllib ml in
-     iter (fun (n, d) ->
-         FStarC_Util.write_file
-           (FStarC_Find.prepend_output_dir (BatString.concat "" [n;ext]))
-           (FStarC_Extraction_ML_Code.pretty (Prims.parse_int "120") d)
-           ) new_doc
+     let p, _ = modul in
+     let n = FStarC_Extraction_ML_Util.flatten_mlpath p in
+     let doc = FStarC_Extraction_ML_Code.doc_of_mlmodule true modul in
+     FStarC_Util.write_file
+       (FStarC_Find.prepend_output_dir (BatString.concat "" [n;ext]))
+       (FStarC_Extraction_ML_Code.pretty (Prims.parse_int "120") doc)
   | _ -> failwith "Unrecognized extension"
