src/extraction/FStarC.Extraction.ML.RemoveUnusedParameters.fst
@@ -330,7 +330,7 @@ let elim_one_mltydecl (env:env_t) (td:one_mltydecl)
     { td with tydecl_parameters = parameters;
               tydecl_defn = body }
 
-let elim_module env m =
+let elim_modulebody env m =
   let elim_module1 env m =
     match m.mlmodule1_m with
     | MLM_Ty td ->
@@ -363,28 +363,24 @@ let set_current_module (e:env_t) (n:mlpath) =
   let curmod = fst n @ [snd n] in
   { e with current_module = curmod }
 
-let elim_mllib (env:env_t) (m:mllib) =
+let elim_mllib (env:env_t) (m:mlmodule) =
   if Options.codegen() <> Some Options.FSharp then env, m else
-  let (MLLib libs) = m in
   let elim_one_lib env lib =
-    let name, sig_mod, _libs = lib in
+    let name, sig_mod = lib in
     let env = set_current_module env name in
     let sig_mod, env =
         match sig_mod with
         | Some (sig_, mod_)  ->
           //intentionally discard the environment from the module translation
-          let env, mod_ = elim_module env mod_ in
+          let env, mod_ = elim_modulebody env mod_ in
           // The sig is currently empty
           Some (sig_, mod_), env
         | None ->
           None, env
     in
-    env, (name, sig_mod, _libs)
+    env, (name, sig_mod)
   in
-  let env, libs =
-    BU.fold_map elim_one_lib env libs
-  in
-  env, MLLib libs
+  elim_one_lib env m
 
-let elim_mllibs (l:list mllib) : list mllib =
+let elim_mllibs (l:list mlmodule) : list mlmodule =
   snd (BU.fold_map elim_mllib initial_env l)
